# Lecture 13 (Tue 11/14/2023)

Owner: Philip Manfred Pincencia

## Joint pdf of 2 random variables satisfies

$$
P((X,Y)\in T)=\iint_T f_{X,Y} (u,v) ~dudv
$$

If $f$ is constant in $T$ and zero elsewhere, we say $f$ is “uniform on $T$”. Assume $f(u,v)=C$ whenever $(u,v)\in T$

In this case we get, 

$$
P((X,Y)\in T)=\iint_T C ~dudv\\=C \iint_Tdudv=C\cdot\text{ Area of }T
$$

*Note: pdfs are not always uniform*

Recall, with discrete random variables: $\sum_{u,v} P_{X,Y}(u,v)=1$. 

But if $X,Y$ are continuous, and we take $T=\mathbb{R}^2$ *(entire plane)*, then we know $P((X,Y)\in T)=1$

$$
\int_{-\infty}^\infty \int_{-\infty}^\infty f_{X,Y}(u,v)~dudv=1
$$

### **Get joint CDF from joint pdf?**

Joint CDF: $F_{X,Y}(u,v)=P(X\leq u, Y\leq v)=P((X,Y)\in T)$
, where 

$$
T=\{(s,t)\in\mathbb{R}^2: s\leq u, t\leq v\} \\ \therefore F_{X,Y}(u,v)=\iint_T f_{X,Y}(s,t)~dsdt=\int_{-\infty}^v\int_{-\infty}^u f_{X,Y} (s,t)~dsdt
$$

### Get Joint pdf from join CDF?

Take derivatives:

1. Take partial derivative w.r.t. $v$
$\frac{\partial}{\partial v}F_{X,Y}(u,v)=\frac{\partial}{\partial v}  \int_{-\infty}^v\left(\int_{-\infty}^u f_{X,Y} (s,t)~ds\right )dt$
Use Leibniz rule ⇒ 2nd & 3rd terms are zero
$=\int_{-\infty}^u f_{X,Y} (s,v)~ds$
2. Now take partial derivative w.r.t. $u$
$\frac{\partial}{\partial u}\frac{\partial}{\partial v}F_{X,Y}(u,v)=\frac{\partial}{\partial u} \int_{-\infty}^u f_{X,Y} (s,t)~ds$
Use Leibniz again ⇒ 2nd & 3rd terms are zero
$=f_{X,Y}(u,v)$ $=$ “joint pdf”
    
    $$
    f_{X,Y}(u,v)=\frac{\partial^2 F_{X,Y(u,v)}}{\partial u \partial v}
    $$
    

Note: You can interchange which you want to differentiate first. 

### Get marginal pdfs from joint pdf?

Suppose $X,Y$ have joint pdf $f_{X,Y}(u,v)$. 

We know 

- $F_{X,Y}(u,v)=\int_{-\infty}^v\int_{-\infty}^u f_{X,Y} (s,t)~dsdt$.
- $F_X(u)=F_{X,Y}(u,\infty)=\int_{-\infty}^\infty \int_{-\infty}^u f_{X,Y} (s,t)~dsdt$

Take derivative of $F_X(u)$ to get pdf: 

$f_X(u)=\frac{d}{du}F_X(u)=\frac{d}{du}\int_{-\infty}^\infty\int_{-\infty}^u f_{X,Y} (s,t)~dsdt$

Use Leibniz again ⇒ 1st and 2nd terms are zero

$=\int_{-\infty}^\infty \frac{d}{du}\int_{-\infty}^u f_{X,Y} (s,t)~dsdt$

Use Leibniz ⇒ 2nd and 3rd terms are zero

$=\int_{-\infty}^\infty \frac{d}{du}f_{X,Y} (u,t)~dsdt$

Rename $t$ to $v$ to look nicer: 

$$
f_X(u)=\int_{-\infty}^\infty f_{X,Y}(u,v)~\bold{dv}\\
f_X(v)=\int_{-\infty}^\infty f_{X,Y}(u,v)~\bold{du}
$$

# Examples

Given $X,Y$ with joint pdf

$$
f_{X,Y}=\begin{cases}       
Ce^{-u} & 0<v<u \\
      0 & \text{else}
      
   \end{cases}
$$

1. What is $C$? 
    
    Using $\int_{-\infty}^\infty \int_{-\infty}^\infty f_{X,Y}(u,v)~dudv=1$. 
    
    Do it both ways: 
    
    Integrate w.r.t. $v$ first (*vertical strips*):
    
     
    
    $$
    \int_0^\infty \int_0^u Ce^{-u}~dvdu=1 \\
    C\int_0^\infty e^{-u} \int_0^u dvdu=C\int_0^\infty ue^{-u} du=C[-ue^{-u}-e^{-u}]_0^\infty=C=1
    $$
    

OR

Integrate w.r.t. $u$ first (*horizontal strips*): 

$$
\int_0^\infty \int_v^\infty Ce^{-u}~dudv=1 \\

$$

1. Find marginal pdfs of $X,Y$: 

$$
f_X(u)=\int_{-\infty}^\infty f_{X,Y}(u,v)~dv=\int_0^u e^{-u}dv=ue^{-u} ~\forall u>0~ (0 \text{ if } u\leq 0) \\
f_Y(v)=\int_{-\infty}^\infty f_{X,Y}(u,v)~du=\int_v^\infty e^{-u}du=e^{-v}~\forall v>0~ (0 \text{ if } v\leq 0)
$$

1. Find $P(X<2Y)$
Rephrase it: $P(X<2Y)=P((X,Y)\in T)$, where $T=\{(u,v): u<2v\}$
    
    We will be integrating from $v$ to $2v$ for the $u$-integrand:
    

$$
=\int_{0}^\infty \int_v^{2v} e^{-u}~dudv=\int_{0}^\infty (e^{-v}-e^{-2v})~dv=\left[-e^{-v}+\frac{1}{2}e^{-2v}\right]_0^\infty=1-\frac{1}{2}=\frac{1}{2}
$$

1. Let $a>0$. Find $P(X+Y\leq a)$
Rephrase: $P(X+Y\leq a)=P((X,Y)\in T)$, where $T=\{(u,v):u+v\leq a\}$
    
    So, $u\leq -v+a$ . The intersection is $(\frac{a}{2}, \frac{a}{2})$. Know $u=v$, so $v+v\leq a\to v\leq \frac{a}{2}$
    
    $$
    =\int_{0}^\frac{a}{2} \int_v^{a-v} e^{-u}~dudv=\int_{0}^\frac{a}{2} (e^{-v}-e^{v-a})~dv=\left[-e^{-v}+e^{v-a}\right]_0^\frac{a}{2}=1-2e^{-\frac{a}{2}}+e^{-a}=(1-e^{-\frac{a}{2}})^2
    $$
    

*Doing it the other way requires us to split into two double integrals*

1. Let $Z=X+Y$. Find $f_Z(w)$
    
    *How?* Find CDF of $Z$ first then differentiate
    
    $$
    F_Z(w)=P(Z\leq w)=P(X+Y\leq w)
    $$
    
    From previous question, 
    
    If $w\leq 0$, $F_Z(w)=0$
    
    If $w>0$, $F_Z(w)=(1-e^{-\frac{w}{2}})^2$
    Hence, 
    
    $$
    f_Z(w)=\frac{d}{dw}F_Z(w)=e^{-\frac{w}{2}}-e^{-w}
    $$