# Lecture 11 (Tue 11/07/2023)

Owner: Philip Manfred Pincencia

## Functions of Random Variables

Goal: If given random variable $X$ and form a random variable $Y$ which is a function of $X$, say $Y=g(X)$. Then, find the pmf or pdf of $Y$. 

Suppose $X$ is discrete uniform on $\{-n, -n+1, …, -1, 0, 1, …, n-1, n\}$. The pmf is $p_X(u)=\frac{1}{2n+1}$ $\forall n\in Z$

Create a new random variable $Y=X^2$. Then, $Y$ takes on values $\{0, 1, 4, 9,…, n^2\}$. The pmf of $Y$ is 

$$
p_Y(u)=P(Y=u)=P(X^2=u)= P(X=\sqrt{u}~\cup~X=-\sqrt{u})= \begin{cases}       \frac{1}{2n+1} & \text{if }u=0 \\
      \frac{2}{2n+1} & \text{else}
   \end{cases}
$$

For general case, 

> If $Y=aX+b$, then $p_Y(u)=p_X(\frac{u-b}{a})$
> 

For continuous random variable, 

To find pdf of 

> If $Y=aX+b$, to find $p_Y(u)$ from $p_X(u)$, we: 
1.  Set up CDF of $Y$: $F_Y(u)$ 
2. Differentiate it
> 

Assume $a>0$,

CDF of $Y$ is: 

1. $F_Y(u)=P(Y\leq u) = P(aX+b\leq u)=P(X\leq\frac{u-b}{a})=F_X(\frac{u-b}{a})$
2. $f_Y(u)=\frac{dF_Y(u)}{du}=\frac{d}{dx}F_X(\frac{u-b}{a})=f_X(\frac{u-b}{a})\cdot \frac{1}{a}$. 

Another way: 

We can write $F_Y(u)=\int_{-\infty}^\frac{u-b}{a}f_X(z)dz$.

The pdf of $Y$ is 

 **Using Leibniz’s Rule:**

$$
f_Y(u)=\frac{d}{du}\int_{-\infty}^\frac{u-b}{a}f_X(z)dz=\frac{1}{a}f_X(\frac{u-b}{a})-\cancel{f_X(-\infty)}
$$

Special case:

For Gaussian, $Y=aX+b$, $X\sim N(\mu, \sigma^2)$

$$
f_Y(u)=\frac{1}{a}f_X(\frac{u-b}{a})=\frac{1}{(a\sigma)\sqrt{2\pi}}e^{-\frac{1}{2}\left(\frac{u-(b+a\mu)}{(a\sigma)}\right)^2} \\ \therefore Y\sim N(b+a\mu, a^2\sigma^2) \\ E[Y]=b+a\mu \text{    and  } \sigma_Y^2=a^2\sigma^2
$$

*This is not true for other $Y=g(x)$.* 

### General fact about variance:

Let $Y=aX+b$. Find $\sigma_Y^2$ in terms of $\sigma_X^2$. 

$Var(Y)=E[Y^2]-(E[Y])^2=a^2E[X^2]+2abE[X]+b^2~-~(aE[X]+b)^2=a^2E[X^2]-a^2(E[X])^2=a^2\sigma_X^2$. 

$\therefore \sigma_Y^2=a^2\sigma_X^2$

### Example

Let $X$ have pdf $f_X(u)$. Let $Y=X^4$. Find $f_Y(u)$. 

*Solution:* 

1. Find CDF of $Y$: $F_Y(u)=P(Y\leq u)=P(X^4\leq u)=P(-\sqrt[4]{u}\leq X\leq \sqrt[4]{u})=F_X(\sqrt[4]{u})-F_X(-\sqrt[4]{u})$
2. Differentiate: $f_Y(u)=\frac{d}{du}F_Y(u)=\frac{1}{4}u^{-\frac{3}{4}}\left(f_X(\sqrt[4]{u})+f_X(-\sqrt[4]{u}\right)$